Start using ind6 and preserved_down for redE

Inductive.v
@@ -12,13 +12,14 @@ Definition is_ind1 :=
 Hypothesis Hind : is_ind1.
 
 Let is_positive := proj1 Hind.
+Definition is_positive1 := is_positive.
 Let has_ind := proj1 (proj2 Hind).
 Let is_ind := proj2 (proj2 Hind).
 
 Definition preserved1 Q :=
   forall x, G (fun x => P x /\ Q x) x -> Q x.
 Definition preserved_with_inv1 Q R :=
-  forall x, G (fun x => P x /\ Q x /\ R x) x -> Q x.
+  forall x, G (fun x => P x /\ Q x /\ R x) x -> R x -> Q x.
 Definition preserved_down1 Q :=
   forall x R, G (fun x => P x /\ R x) x -> Q x -> G (fun x => P x /\ Q x /\ R x) x.
 
@@ -37,7 +38,7 @@ Lemma preserved_with_inv1_rec :
   forall Q R, preserved_down1 R -> preserved_with_inv1 Q R -> forall x, P x -> R x -> Q x.
 Proof.
   intros Q R H1 H2. refine (preserved1_rec (fun x => R x -> Q x) _).
-  intros x H3 H4. apply H2.
+  intros x H3 H4. apply H2; [|assumption].
   apply is_positive with (Q := fun x => P x /\ R x /\ (R x -> Q x)); [intros; tauto|].
   apply H1; assumption.
 Qed.
@@ -50,11 +51,13 @@ Proof.
   simpl. intros; tauto.
 Qed.
 
+End Ind1.
+
 Ltac prove_ind1 :=
   unfold is_ind1;
   match goal with [ |- ?G1_ /\ ?G2_ /\ ?G3_ ] =>
     pose (G1 := G1_);
-    pose (Hmap := (ltac:(intros Q R H x Hx; destruct Hx; constructor; try assumption; apply H; assumption) : G1));
+    pose (Hmap := (ltac:(intros Q R H x Hx; destruct Hx; econstructor; try eassumption; eapply H; eassumption) : G1));
     split; [exact Hmap|];
     split; [|intros x Hx; constructor; assumption];
     intros Q HQ; fix H 2; intros x Hx;
@@ -62,7 +65,6 @@ Ltac prove_ind1 :=
     apply (Hmap _ Q) in Hx; [apply HQ; assumption|assumption]
   end.
 
-End Ind1.
 
 Section Ind2.
 
@@ -81,13 +83,14 @@ Definition is_ind2 :=
 Hypothesis Hind : is_ind2.
 
 Let is_positive := proj1 Hind.
+Definition is_positive2 := is_positive.
 Let has_ind := proj1 (proj2 Hind).
 Let is_ind := proj2 (proj2 Hind).
 
 Definition preserved2 Q :=
   forall x y, G (fun x y => P x y /\ Q x y) x y -> Q x y.
 Definition preserved_with_inv2 Q R :=
-  forall x y, G (fun x y => P x y /\ Q x y /\ R x y) x y -> Q x y.
+  forall x y, G (fun x y => P x y /\ Q x y /\ R x y) x y -> R x y -> Q x y.
 Definition preserved_down2 Q :=
   forall x y R, G (fun x y => P x y /\ R x y) x y -> Q x y -> G (fun x y => P x y /\ Q x y /\ R x y) x y.
 
@@ -106,7 +109,7 @@ Lemma preserved_with_inv2_rec :
   forall Q R, preserved_down2 R -> preserved_with_inv2 Q R -> forall x y, P x y -> R x y -> Q x y.
 Proof.
   intros Q R H1 H2. refine (preserved2_rec (fun x y => R x y -> Q x y) _).
-  intros x y H3 H4. apply H2.
+  intros x y H3 H4. apply H2; [|assumption].
   apply is_positive with (Q := fun x y => P x y /\ R x y /\ (R x y -> Q x y)); [intros; tauto|].
   apply H1; assumption.
 Qed.
@@ -119,19 +122,19 @@ Proof.
   simpl. intros; tauto.
 Qed.
 
+End Ind2.
+
 Ltac prove_ind2 :=
   unfold is_ind2;
   match goal with [ |- ?G1_ /\ ?G2_ /\ ?G3_ ] =>
     pose (G1 := G1_);
-    pose (Hmap := (ltac:(intros Q R H x y Hxy; destruct Hxy; constructor; try assumption; apply H; assumption) : G1));
+    pose (Hmap := (ltac:(intros Q R H x y Hxy; destruct Hxy; econstructor; try eassumption; eapply H; eassumption) : G1));
     split; [exact Hmap|];
     split; [|intros x y Hxy; constructor; assumption];
     intros Q HQ; fix H 3; intros x y Hxy;
     destruct Hxy as [x1 y1 Hxy];
     apply (Hmap _ Q) in Hxy; [apply HQ; assumption|assumption]
   end.
-
-End Ind2.
 
 
 Section Ind3.
@@ -152,13 +155,14 @@ Definition is_ind3 :=
 Hypothesis Hind : is_ind3.
 
 Let is_positive := proj1 Hind.
+Definition is_positive3 := is_positive.
 Let has_ind := proj1 (proj2 Hind).
 Let is_ind := proj2 (proj2 Hind).
 
 Definition preserved3 Q :=
   forall x y z, G (fun x y z => P x y z /\ Q x y z) x y z -> Q x y z.
 Definition preserved_with_inv3 Q R :=
-  forall x y z, G (fun x y z => P x y z /\ Q x y z /\ R x y z) x y z -> Q x y z.
+  forall x y z, G (fun x y z => P x y z /\ Q x y z /\ R x y z) x y z -> R x y z -> Q x y z.
 Definition preserved_down3 Q :=
   forall x y z R, G (fun x y z => P x y z /\ R x y z) x y z -> Q x y z -> G (fun x y z => P x y z /\ Q x y z /\ R x y z) x y z.
 
@@ -177,7 +181,7 @@ Lemma preserved_with_inv3_rec :
   forall Q R, preserved_down3 R -> preserved_with_inv3 Q R -> forall x y z, P x y z -> R x y z -> Q x y z.
 Proof.
   intros Q R H1 H2. refine (preserved3_rec (fun x y z => R x y z -> Q x y z) _).
-  intros x y z H3 H4. apply H2.
+  intros x y z H3 H4. apply H2; [|assumption].
   apply is_positive with (Q := fun x y z => P x y z /\ R x y z /\ (R x y z -> Q x y z)); [intros; tauto|].
   apply H1; assumption.
 Qed.
@@ -190,19 +194,19 @@ Proof.
   simpl. intros; tauto.
 Qed.
 
+End Ind3.
+
 Ltac prove_ind3 :=
   unfold is_ind3;
   match goal with [ |- ?G1_ /\ ?G2_ /\ ?G3_ ] =>
     pose (G1 := G1_);
-    pose (Hmap := (ltac:(intros Q R H x y z Hxyz; destruct Hxyz; constructor; try assumption; apply H; assumption) : G1));
+    pose (Hmap := (ltac:(intros Q R H x y z Hxyz; destruct Hxyz; econstructor; try eassumption; eapply H; eassumption) : G1));
     split; [exact Hmap|];
     split; [|intros x y z Hxyz; constructor; assumption];
     intros Q HQ; fix H 4; intros x y z Hxyz;
     destruct Hxyz as [x1 y1 z1 Hxyz];
     apply (Hmap _ Q) in Hxyz; [apply HQ; assumption|assumption]
   end.
-
-End Ind3.
 
 
 Section Ind4.
@@ -224,13 +228,14 @@ Definition is_ind4 :=
 Hypothesis Hind : is_ind4.
 
 Let is_positive := proj1 Hind.
+Definition is_positive4 := is_positive.
 Let has_ind := proj1 (proj2 Hind).
 Let is_ind := proj2 (proj2 Hind).
 
 Definition preserved4 Q :=
   forall x y z u, G (fun x y z u => P x y z u /\ Q x y z u) x y z u -> Q x y z u.
 Definition preserved_with_inv4 Q R :=
-  forall x y z u, G (fun x y z u => P x y z u /\ Q x y z u /\ R x y z u) x y z u -> Q x y z u.
+  forall x y z u, G (fun x y z u => P x y z u /\ Q x y z u /\ R x y z u) x y z u -> R x y z u -> Q x y z u.
 Definition preserved_down4 Q :=
   forall x y z u R, G (fun x y z u => P x y z u /\ R x y z u) x y z u -> Q x y z u -> G (fun x y z u => P x y z u /\ Q x y z u /\ R x y z u) x y z u.
 
@@ -249,7 +254,7 @@ Lemma preserved_with_inv4_rec :
   forall Q R, preserved_down4 R -> preserved_with_inv4 Q R -> forall x y z u, P x y z u -> R x y z u -> Q x y z u.
 Proof.
   intros Q R H1 H2. refine (preserved4_rec (fun x y z u => R x y z u -> Q x y z u) _).
-  intros x y z u H3 H4. apply H2.
+  intros x y z u H3 H4. apply H2; [|assumption].
   apply is_positive with (Q := fun x y z u => P x y z u /\ R x y z u /\ (R x y z u -> Q x y z u)); [intros; tauto|].
   apply H1; assumption.
 Qed.
@@ -262,19 +267,19 @@ Proof.
   simpl. intros; tauto.
 Qed.
 
+End Ind4.
+
 Ltac prove_ind4 :=
   unfold is_ind4;
   match goal with [ |- ?G1_ /\ ?G2_ /\ ?G3_ ] =>
     pose (G1 := G1_);
-    pose (Hmap := (ltac:(intros Q R H x y z u Hxyzu; destruct Hxyzu; constructor; try assumption; apply H; assumption) : G1));
+    pose (Hmap := (ltac:(intros Q R H x y z u Hxyzu; destruct Hxyzu; econstructor; try eassumption; eapply H; eassumption) : G1));
     split; [exact Hmap|];
     split; [|intros x y z u Hxyzu; constructor; assumption];
     intros Q HQ; fix H 5; intros x y z u Hxyzu;
     destruct Hxyzu as [x1 y1 z1 u1 Hxyzu];
     apply (Hmap _ Q) in Hxyzu; [apply HQ; assumption|assumption]
   end.
-
-End Ind4.
 
 
 Section Ind5.
@@ -297,13 +302,14 @@ Definition is_ind5 :=
 Hypothesis Hind : is_ind5.
 
 Let is_positive := proj1 Hind.
+Definition is_positive5 := is_positive.
 Let has_ind := proj1 (proj2 Hind).
 Let is_ind := proj2 (proj2 Hind).
 
 Definition preserved5 Q :=
   forall x y z u v, G (fun x y z u v => P x y z u v /\ Q x y z u v) x y z u v -> Q x y z u v.
 Definition preserved_with_inv5 Q R :=
-  forall x y z u v, G (fun x y z u v => P x y z u v /\ Q x y z u v /\ R x y z u v) x y z u v -> Q x y z u v.
+  forall x y z u v, G (fun x y z u v => P x y z u v /\ Q x y z u v /\ R x y z u v) x y z u v -> R x y z u v -> Q x y z u v.
 Definition preserved_down5 Q :=
   forall x y z u v R, G (fun x y z u v => P x y z u v /\ R x y z u v) x y z u v -> Q x y z u v -> G (fun x y z u v => P x y z u v /\ Q x y z u v /\ R x y z u v) x y z u v.
 
@@ -322,7 +328,7 @@ Lemma preserved_with_inv5_rec :
   forall Q R, preserved_down5 R -> preserved_with_inv5 Q R -> forall x y z u v, P x y z u v -> R x y z u v -> Q x y z u v.
 Proof.
   intros Q R H1 H2. refine (preserved5_rec (fun x y z u v => R x y z u v -> Q x y z u v) _).
-  intros x y z u v H3 H4. apply H2.
+  intros x y z u v H3 H4. apply H2; [|assumption].
   apply is_positive with (Q := fun x y z u v => P x y z u v /\ R x y z u v /\ (R x y z u v -> Q x y z u v)); [intros; tauto|].
   apply H1; assumption.
 Qed.
@@ -335,19 +341,19 @@ Proof.
   simpl. intros; tauto.
 Qed.
 
+End Ind5.
+
 Ltac prove_ind5 :=
   unfold is_ind5;
   match goal with [ |- ?G1_ /\ ?G2_ /\ ?G3_ ] =>
     pose (G1 := G1_);
-    pose (Hmap := (ltac:(intros Q R H x y z u v Hxyzuv; destruct Hxyzuv; constructor; try assumption; apply H; assumption) : G1));
+    pose (Hmap := (ltac:(intros Q R H x y z u v Hxyzuv; destruct Hxyzuv; econstructor; try eassumption; eapply H; eassumption) : G1));
     split; [exact Hmap|];
     split; [|intros x y z u v Hxyzuv; constructor; assumption];
     intros Q HQ; fix H 6; intros x y z u v Hxyzuv;
     destruct Hxyzuv as [x1 y1 z1 u1 v1 Hxyzuv];
     apply (Hmap _ Q) in Hxyzuv; [apply HQ; assumption|assumption]
   end.
-
-End Ind5.
 
 
 Section Ind6.
@@ -371,13 +377,14 @@ Definition is_ind6 :=
 Hypothesis Hind : is_ind6.
 
 Let is_positive := proj1 Hind.
+Definition is_positive6 := is_positive.
 Let has_ind := proj1 (proj2 Hind).
 Let is_ind := proj2 (proj2 Hind).
 
 Definition preserved6 Q :=
   forall x y z u v w, G (fun x y z u v w => P x y z u v w /\ Q x y z u v w) x y z u v w -> Q x y z u v w.
 Definition preserved_with_inv6 Q R :=
-  forall x y z u v w, G (fun x y z u v w => P x y z u v w /\ Q x y z u v w /\ R x y z u v w) x y z u v w -> Q x y z u v w.
+  forall x y z u v w, G (fun x y z u v w => P x y z u v w /\ Q x y z u v w /\ R x y z u v w) x y z u v w -> R x y z u v w -> Q x y z u v w.
 Definition preserved_down6 Q :=
   forall x y z u v w R, G (fun x y z u v w => P x y z u v w /\ R x y z u v w) x y z u v w -> Q x y z u v w -> G (fun x y z u v w => P x y z u v w /\ Q x y z u v w /\ R x y z u v w) x y z u v w.
 
@@ -396,7 +403,7 @@ Lemma preserved_with_inv6_rec :
   forall Q R, preserved_down6 R -> preserved_with_inv6 Q R -> forall x y z u v w, P x y z u v w -> R x y z u v w -> Q x y z u v w.
 Proof.
   intros Q R H1 H2. refine (preserved6_rec (fun x y z u v w => R x y z u v w -> Q x y z u v w) _).
-  intros x y z u v w H3 H4. apply H2.
+  intros x y z u v w H3 H4. apply H2; [|assumption].
   apply is_positive with (Q := fun x y z u v w => P x y z u v w /\ R x y z u v w /\ (R x y z u v w -> Q x y z u v w)); [intros; tauto|].
   apply H1; assumption.
 Qed.
@@ -409,24 +416,19 @@ Proof.
   simpl. intros; tauto.
 Qed.
 
+End Ind6.
+
 Ltac prove_ind6 :=
   unfold is_ind6;
   match goal with [ |- ?G1_ /\ ?G2_ /\ ?G3_ ] =>
     pose (G1 := G1_);
-    pose (Hmap := (ltac:(intros Q R H x y z u v w Hxyzuvw; destruct Hxyzuvw; constructor; try assumption; apply H; assumption) : G1));
+    pose (Hmap := (ltac:(intros Q R H x y z u v w Hxyzuvw; destruct Hxyzuvw; econstructor; try eassumption; eapply H; eassumption) : G1));
     split; [exact Hmap|];
     split; [|intros x y z u v w Hxyzuvw; constructor; assumption];
     intros Q HQ; fix H 7; intros x y z u v w Hxyzuvw;
     destruct Hxyzuvw as [x1 y1 z1 u1 v1 w1 Hxyzuvw];
     apply (Hmap _ Q) in Hxyzuvw; [apply HQ; assumption|assumption]
   end.
-
-End Ind6.
-
-
-
-
-
 
 
 
@@ -446,18 +448,6 @@ Inductive test (rec : nat -> nat -> Prop) : nat -> nat -> Prop :=
 Inductive t : nat -> nat -> Prop :=
 | t_intro : forall n m, test t n m -> t n m.
 
-Ltac prove_ind2 :=
-  unfold is_ind2;
-  match goal with [ |- ?G1_ /\ ?G2_ /\ ?G3_ ] =>
-    pose (G1 := G1_);
-    pose (Hmap := (ltac:(intros Q R H x y Hxy; destruct Hxy; constructor; try assumption; apply H; assumption) : G1));
-    split; [exact Hmap|];
-    split; [|intros x y Hxy; constructor; assumption];
-    intros Q HQ; fix H 3; intros x y Hxy;
-    destruct Hxy as [x1 y1 Hxy];
-    apply (Hmap _ Q) in Hxy; [apply HQ; assumption|assumption]
-  end.
-
 Lemma t_ind2 : is_ind2 test t.
 Proof. prove_ind2. Qed.
 
@@ -475,4 +465,5 @@ Proof.
   - assumption.
   - simpl. constructor. constructor. tauto.
 Qed.
+
 *)
